SSA/Experimental/Bits/Fast/Profile.lean
@@ -13,7 +13,7 @@ Authors: Siddharth Bhat
 -/
 import SSA.Experimental.Bits.Fast.Reflect
 import Lean
-open Lean 
+open Lean
 
 open Lean Elab Meta
 #check Lean.Core.CoreM.toIO
@@ -50,17 +50,17 @@ open Std Sat AIG in
 Convert a 'Circuit α' into an 'AIG α' in order to reuse bv_decide's
 bitblasting capabilities.
 -/
-def Circuit.toAIG [DecidableEq α] [Fintype α] [Hashable α] (c : Circuit α) (aig : AIG α) : 
+def Circuit.toAIG [DecidableEq α] [Fintype α] [Hashable α] (c : Circuit α) (aig : AIG α) :
     ExtendingEntrypoint aig :=
-  match c with 
+  match c with
   | .fals => ⟨aig.mkConstCached false, by apply  LawfulOperator.le_size⟩
   | .tru => ⟨aig.mkConstCached true, by apply  LawfulOperator.le_size⟩
-  | .var b v => 
+  | .var b v =>
     let out := mkAtomCached aig v
     have AtomLe := LawfulOperator.le_size (f := mkAtomCached) aig v
     if b then
       ⟨out, by simp [out]; omega⟩
-    else 
+    else
       let notOut := mkNotCached out.aig out.ref
       have NotLe := LawfulOperator.le_size (f := mkNotCached) out.aig out.ref
       ⟨notOut, by simp only [notOut, out] at NotLe AtomLe ⊢; omega⟩
@@ -74,7 +74,7 @@ def Circuit.toAIG [DecidableEq α] [Fintype α] [Hashable α] (c : Circuit α) (
     let ret := aig.mkAndCached input
     have Lawful := LawfulOperator.le_size (f := mkAndCached) aig input
     ⟨ret, by dsimp only [ret] at lextend rextend ⊢; omega⟩
-  | .or l r => 
+  | .or l r =>
     let ⟨⟨aig, lhsRef⟩, lextend⟩ := l.toAIG aig
     let ⟨⟨aig, rhsRef⟩, rextend⟩ := r.toAIG aig
     let lhsRef := lhsRef.cast <| by
@@ -84,7 +84,7 @@ def Circuit.toAIG [DecidableEq α] [Fintype α] [Hashable α] (c : Circuit α) (
     let ret := aig.mkOrCached input
     have Lawful := LawfulOperator.le_size (f := mkOrCached) aig input
     ⟨ret, by dsimp only [ret] at lextend rextend ⊢; omega⟩
-  | .xor l r => 
+  | .xor l r =>
     let ⟨⟨aig, lhsRef⟩, lextend⟩ := l.toAIG aig
     let ⟨⟨aig, rhsRef⟩, rextend⟩ := r.toAIG aig
     let lhsRef := lhsRef.cast <| by
@@ -95,6 +95,135 @@ def Circuit.toAIG [DecidableEq α] [Fintype α] [Hashable α] (c : Circuit α) (
     have Lawful := LawfulOperator.le_size (f := mkXorCached) aig input
     ⟨ret, by dsimp only [ret] at lextend rextend ⊢; omega⟩
 
+open Std Sat AIG Tactic BVDecide Frontend in
+def TacticContext.new (lratPath : System.FilePath) (config : BVDecideConfig) :
+    TermElabM TacticContext := do
+  -- Account for: https://github.com/arminbiere/cadical/issues/112
+  let config :=
+    if System.Platform.isWindows then
+      { config with binaryProofs := false }
+    else
+      config
+  let exprDef ← Lean.Elab.Term.mkAuxName `_expr_def
+  let certDef ← Lean.Elab.Term.mkAuxName `_cert_def
+  let reflectionDef ← Lean.Elab.Term.mkAuxName `_reflection_def
+  let solver ← determineSolver
+  trace[Meta.Tactic.sat] m!"Using SAT solver at '{solver}'"
+  return {
+    exprDef,
+    certDef,
+    reflectionDef,
+    solver,
+    lratPath,
+    config
+  }
+where
+  determineSolver : Lean.Elab.TermElabM System.FilePath := do
+    let opts ← getOptions
+    let option := sat.solver.get opts
+    if option == "" then
+      let cadicalPath := (← IO.appPath).parent.get! / "cadical" |>.withExtension System.FilePath.exeExtension
+      if ← cadicalPath.pathExists then
+        return cadicalPath
+      else
+        return "cadical"
+    else
+      return option
+
+
+open Std Sat AIG Tactic BVDecide Frontend in
+def checkCircuitTautoAux [DecidableEq α] [Hashable α] [Fintype α] (c : Circuit α) : TermElabM Bool := do
+  let cfg : BVDecideConfig := {}
+  IO.FS.withTempFile fun _ lratFile => do
+    let cfg ← BVDecide.Frontend.TacticContext.new lratFile cfg
+    let c := c.not -- we're checking TAUTO, so check that negation is UNSAT.
+    let ⟨entrypoint, hEntrypoint⟩ := c.toAIG AIG.empty
+    let ⟨entrypoint, labelling⟩ := entrypoint.relabelNat'
+    let cnf := toCNF entrypoint
+    let out ← runExternal cnf cfg.solver cfg.lratPath (trimProofs := true) (timeout := 1000) (binaryProofs := true)
+    match out with 
+    | .error _model => return false 
+    | .ok _cert => return true
+
+
+def Circuit.decLeCadical {α : Type} [DecidableEq α] [Fintype α]
+  (c : Circuit α) (c' : Circuit α) : TermElabM { b : Bool // b ↔ c ≤ c' } := do 
+ -- Justified by Circuit.le_iff_implies 
+ let impliesCircuit := c.implies c'
+ checkCircuitTautoAux impliesCircuit
+
+/-- 
+An axiom that tracks that a theorem is true because of our currently unverified
+'decideIfZerosM' decision procedure.
+-/
+axiom decideIfZerosMAx {p : Prop} : p
+/--
+Reflect an expression of the form:
+  ∀ ⟦(w : Nat)⟧ (← focus)
+  ∀ (b₁ b₂ ... bₙ : BitVec w),
+  <proposition about bitvectors>.
+
+Reflection code adapted from `elabNaticeDecideCoreUnsafe`,
+which explains how to create the correct auxiliary definition of the form
+`decideProprerty = true`, such that our goal state after using `ofReduceBool` becomes
+⊢ ofReduceBool decideProperty = true
+
+which is then indeed `rfl` equal to `true`.
+-/
+def reflectUniversalWidthBVsWithCadical (g : MVarId) : TermElabM (List MVarId) := do
+  let ws ← Reflect.findExprBitwidths (← g.getType)
+  let ws := ws.toArray
+  if h0: ws.size = 0 then throwError "found no bitvector in the target: {indentD (← g.getType)}"
+  else if hgt: ws.size > 1 then
+    let (w1, wExample1) := ws[0]
+    let (w2, wExample2) := ws[1]
+    let mExample := f!"{w1} → {wExample1}" ++ f!"{w2} → {wExample2}"
+    throwError "found multiple bitvector widths in the target: {indentD mExample}"
+  else
+    -- we have exactly one width
+    let (w, wExample) := ws[0]
+
+    -- We can now revert hypotheses that are of this bitwidth.
+    let g ← Reflect.revertBvHyps g
+
+    -- Next, after reverting, we have a goal which we want to reflect.
+    -- we convert this goal to NNF
+    let .some g ← NNF.runNNFSimpSet g
+      | logInfo m!"Converting to negation normal form automatically closed goal."
+        return[]
+    logInfo m!"goal after NNF: {indentD g}"
+
+    let .some g ← Simplifications.runPreprocessing g
+      | logInfo m!"Preprocessing automatically closed goal."
+        return[]
+    logInfo m!"goal after preprocessing: {indentD g}"
+
+    -- finally, we perform reflection.
+    let result ← Reflect.reflectPredicateAux ∅ (← g.getType) w
+    result.bvToIxMap.throwWarningIfUninterpretedExprs
+
+    logInfo m!"predicate (repr): {indentD (repr result.e)}"
+
+    let bvToIxMapVal ← result.bvToIxMap.toExpr w
+
+    let target := (mkAppN (mkConst ``Predicate.denote) #[result.e.quote, w, bvToIxMapVal])
+    let g ← g.replaceTargetDefEq target
+    logInfo m!"goal after reflection: {indentD g}"
+
+    -- Log the finite state machine size, and bail out if we cross the barrier.
+    let fsm := predicateEvalEqFSM result.e |>.toFSM 
+    let isTrueForall ← decideIfZerosM Circuit.decLeCadical fsm
+    if isTrueForall
+    then do
+      let gs ← g.apply (mkConst ``decideIfZerosMAx [])
+      if gs.isEmpty
+      then return gs
+      else 
+        throwError "Expected application of 'decideIfZerosMAx' to close goal, but failed. {indentD g}"
+    else
+      throwError "failed to prove goal, since decideIfZerosM established that theorem is not true."
+      return [g]
+      
 
 /-!
 We disable closed term extraction to make sure that the evaluation of
